utils/choreoUtilsScript.sml
@@ -1,0 +1,33 @@
+open preamble
+
+val _ = new_theory "choreoUtils";
+
+
+Theorem RTC_TRANS = RTC_RULES |> CONV_RULE FORALL_AND_CONV
+                              |> CONJUNCTS |> el 2;
+
+
+(* Alternative version of nub that keeps elements at the
+   head of the list
+*)
+Definition nub'_def:
+  nub' []      = []
+∧ nub' (x::xs) = x :: FILTER ($≠ x) (nub' xs)
+Termination
+  WF_REL_TAC `measure LENGTH`
+  \\ rw [LENGTH]
+  \\ ho_match_mp_tac LESS_EQ_LESS_TRANS
+  \\ Q.EXISTS_TAC `LENGTH xs`
+  \\ rw [LENGTH_FILTER_LEQ]
+End
+
+(* lists produced by nub' are ALL_DISTINCT *)
+Theorem all_distinct_nub':
+  ∀l. ALL_DISTINCT (nub' l)
+Proof
+  rw [ALL_DISTINCT,nub'_def]
+  \\ Induct_on `l`
+  \\ rw [ALL_DISTINCT,nub'_def,FILTER_ALL_DISTINCT,MEM_FILTER]
+QED
+
+val _ = export_theory ()
